x86/SelectLongproof.v
@@ -331,7 +331,7 @@ Proof.
   { intros. replace (Ptrofs.repr n) with (Ptrofs.of_int64 (Int64.repr n)) by auto with ptrofs.
     apply Genv.shift_symbol_address_64; auto. }
   unfold addl. destruct Archi.splitlong eqn:SL.
-  apply SplitLongproof.eval_addl. apply Archi.splitlong_ptr32; auto.
+  apply SplitLongproof.eval_addl. auto.
   red; intros; destruct (addl_match a b); InvEval.
 - rewrite Val.addl_commut. apply eval_addlimm; auto.
 - apply eval_addlimm; auto.
@@ -353,7 +353,7 @@ Qed.
 Theorem eval_subl: binary_constructor_sound subl Val.subl.
 Proof.
   unfold subl. destruct Archi.splitlong eqn:SL.
-  apply SplitLongproof.eval_subl. apply Archi.splitlong_ptr32; auto.
+  apply SplitLongproof.eval_subl. auto.
   red; intros; destruct (subl_match a b); InvEval.
 - rewrite Val.subl_addl_opp. apply eval_addlimm; auto.
 - subst. rewrite Val.subl_addl_l. rewrite Val.subl_addl_r.
